messing with isLrPair

theories/LogicalRelation/Introductions/Sigma.v
@@ -9,10 +9,20 @@ Section SigmaRed.
 
 Context `{GenericTypingProperties}.
 
-Lemma redΣdom {Γ F F' G G' l} : [Γ ||-S<l> tSig F G ≅ tSig F' G'] -> [Γ ||-S<l> F ≅ F'].
+Lemma SredΣdom {Γ F F' G G' l} : [Γ ||-S<l> tSig F G ≅ tSig F' G'] -> [Γ ||-S<l> F ≅ F'].
 Proof.
   intros RΣ0; unshelve eapply (SinstKripke _ (normRedΣ RΣ0).(PolyRed.shpRed)).
   escape; gtyping.
+Qed.
+
+
+Lemma redΣdom {Γ} {wfΓ :[|-Γ]} {F F' G G' l} : [wfΓ ||-<l> tSig F G ≅ tSig F' G'] -> [wfΓ ||-<l> F ≅ F'].
+Proof.
+  intros RΣ.
+  eapply (Split_bind_return RΣ).
+  intros ??? oRΣ.
+  eapply SredΣdom.
+  now eapply RΣ.
 Qed.
 
 Lemma redΣcod {Γ} {wfΓ :[|-Γ]} {F} {wfF : [Γ |- F]} {F' G G' l} : [Γ ||-S<l> tSig F G ≅ tSig F' G'] -> [wfc_cons wfΓ wfF ||-<l> G ≅ G'].
@@ -25,7 +35,7 @@ Lemma redΣcodfst {Γ} {wfΓ :[|-Γ]} {F F' G G' l} (RΣ: [Γ ||-S<l> tSig F G �
 Proof.
   intros Ra.
   unshelve now eapply (instKripkeSubst wfΓ (normRedΣ RΣ).(PolyRed.posRed)); eapply SirrLR.
-  apply (redΣdom (LRSig' (normRedΣ RΣ))).
+  apply (SredΣdom (LRSig' (normRedΣ RΣ))).
 Qed.
 
 
@@ -33,7 +43,7 @@ Import SigRedTmEq.
 
 Lemma isLRPair_isWfPair {Γ A A' B B' l p} (ΣA : [Γ ||-S<l> tSig A B ≅ tSig A' B'])
   (RΣ := (normRedΣ ΣA))
-  (Rp : isLRPair' RΣ p) :
+  (Rp : isLRPair RΣ p) :
     isWfPair Γ A B p.
 Proof.
   assert (wfΓ: [|- Γ]) by (escape ; gen_typing).
@@ -51,16 +61,15 @@ Qed.
 
 Section Helpers.
 Context {Γ l A A'} (RA : [Γ ||-Σ<l> A ≅ A'])
-  {t u} (Rt : SigRedTm' RA t) (Ru : SigRedTm' RA u).
+  {t u} (Rt : SigRedTm RA t) (Ru : SigRedTm RA u).
 
 Lemma build_sigRedTmEq
-  (eqnf : [Γ |- Rt.(SigRedTmEq'.nf) ≅ Ru.(SigRedTmEq'.nf) : ParamRedTy.outTyL RA])
+  (eqnf : [Γ |- Rt.(SigRedTmEq.nf) ≅ Ru.(SigRedTmEq.nf) : ParamRedTy.outTyL RA])
   (wfΓ : [|- Γ])
-  (Rfst : [ SinstKripke wfΓ RA.(PolyRed.shpRed) | _ ||- tFst Rt.(SigRedTmEq'.nf) ≅ tFst Ru.(SigRedTmEq'.nf) : _ ])
-  (Rsnd : [ instKripkeSubst wfΓ RA.(PolyRed.posRed) _ Rfst | _ ||- tSnd Rt.(SigRedTmEq'.nf) ≅ tSnd Ru.(SigRedTmEq'.nf) : _ ]) :
+  (Rfst : [ SinstKripke wfΓ RA.(PolyRed.shpRed) | _ ||- tFst Rt.(nf) ≅ tFst Ru.(nf) : _ ])
+  (Rsnd : [ instKripkeSubst wfΓ RA.(PolyRed.posRed) _ Rfst | _ ||- tSnd Rt.(nf) ≅ tSnd Ru.(nf) : _ ]) :
   [LRSig' RA | _ ||- t ≅ u : _].
 Proof.
-  eapply SigRedTmEq_to.
   unshelve eexists Rt Ru _; tea.
   - intros; now unshelve now eapply SirrLR; rewrite 2!wk_fst; eapply SwkLR.
   - intros; eapply irrLREq.
@@ -91,11 +100,11 @@ End Helpers.
 Lemma build_sigRedTmEq' {Γ} {wfΓ :[|-Γ]} {l F F' G G'}
   (RΣ0 : [Γ ||-S<l> tSig F G ≅ tSig F' G'])
   (RΣ := normRedΣ RΣ0)
-  {t u} (Rt : SigRedTm' RΣ t) (Ru : SigRedTm' RΣ u)
-  (Rdom := redΣdom RΣ0)
-  (Rfst : [ Rdom | _ ||- tFst Rt.(SigRedTmEq'.nf) ≅ tFst Ru.(SigRedTmEq'.nf) : _ ])
+  {t u} (Rt : SigRedTm RΣ t) (Ru : SigRedTm RΣ u)
+  (Rdom := SredΣdom RΣ0)
+  (Rfst : [ Rdom | _ ||- tFst Rt.(nf) ≅ tFst Ru.(nf) : _ ])
   (Rcod := instKripkeSubst wfΓ RΣ.(PolyRed.posRed) _ Rfst)
-  (Rsnd : [ Rcod | _ ||- tSnd Rt.(SigRedTmEq'.nf) ≅ tSnd Ru.(SigRedTmEq'.nf) : _ ]) :
+  (Rsnd : [ Rcod | _ ||- tSnd Rt.(nf) ≅ tSnd Ru.(nf) : _ ]) :
   [LRSig' RΣ | _ ||- t ≅ u : _].
 Proof.
   unshelve eapply (build_sigRedTmEq _ Rt Ru).
@@ -104,11 +113,45 @@ Proof.
   2: eapply irrLREq; tea; reflexivity.
   epose proof (redΣcod RΣ0); escape.
   eapply convtm_eta_sig; cbn -[Wpack] in *; tea; destruct Rt, Ru; cbn -[Wpack] in *.
-  2: eapply isLRPair_isWfPair.
   all: first [now eapply isLRPair_isWfPair| gtyping].
   Unshelve.
   eapply wfΓ.
   now eapply escape.
+Qed.
+
+Lemma canonSig {Γ A A' B B' l p p'}
+  {RΣ : [Γ ||-S< l > tSig A B ≅ tSig A' B']} :
+  [ Γ ||-S< l > p ≅ p' : tSig A B | RΣ] ->
+  [ Γ ||-S< l > p ≅ p' : tSig A B | LRSig' (normRedΣ RΣ)].
+Proof.
+  intro. now eapply SirrLR.
+Qed.
+
+Lemma canonSig_inv {Γ A A' B B' l p p'}
+  {RΣ : [Γ ||-S< l > tSig A B ≅ tSig A' B']} :
+  [ Γ ||-S< l > p ≅ p' : tSig A B | LRSig' (normRedΣ RΣ)] ->
+  [ Γ ||-S< l > p ≅ p' : tSig A B | RΣ].
+Proof.
+  intro. now eapply SirrLR.
+Qed.
+
+Lemma SfstRed {l Γ F F' G G' p p'}
+  (RΣ : [Γ ||-S<l> tSig F G ≅ tSig F' G'])
+  (RF : [Γ ||-S<l> F ≅ F'])
+  (Rp : [Γ ||-S<l> p ≅ p' : _ | RΣ]) :
+  [Γ ||-S<l> tFst p ≅ tFst p' : _ | RF].
+Proof.
+  eassert (wfΓ:[|-Γ]) by (escape; gtyping).
+  eapply (SirrLR (LRSig' (normRedΣ RΣ))) in Rp.
+  eapply SredSubstTmEq; cycle 1.
+  + eapply redtm_fst, tmr_wf_red. exact (SigRedTmEq.red (SigRedTmEq.redL Rp)).
+  + eapply redtm_fst, tmr_wf_red.
+    eapply redtmwf_conv.
+    1:exact (SigRedTmEq.red (SigRedTmEq.redR Rp)).
+    now escape.
+  + epose proof (SigRedTmEq.eqFst Rp wk_id wfΓ) as Rp'.
+    erewrite 2!wk_id_ren_on in Rp'.
+    eapply SirrLREq with (1:= wk_id_ren_on _ _), Rp'.
 Qed.
 
 Lemma fstRed {l Γ} {wfΓ : [|-Γ]} {F F' G G' p p'}
@@ -117,29 +160,13 @@ Lemma fstRed {l Γ} {wfΓ : [|-Γ]} {F F' G G' p p'}
   (Rp : [Γ ||-S<l> p ≅ p' : _ | RΣ]) :
   [wfΓ ||-<l> tFst p ≅ tFst p' : _ | RF].
 Proof.
-  eapply (SirrLR (LRSig' (normRedΣ RΣ))) in Rp.
-  eapply redSubstTmEq; cycle 1.
-  + eapply redtm_fst, tmr_wf_red. exact (SigRedTmEq.red (SigRedTmEq.redL Rp)).
-  + eapply redtm_fst, tmr_wf_red.
-    eapply redtmwf_conv.
-    1:exact (SigRedTmEq.red (SigRedTmEq.redR Rp)).
-    now escape.
-  + eapply Split_return; intros ??? oRF.
-    now unshelve eapply SirrLR, (SigRedTmEq.eqFst Rp).
+  eapply Split_return.
+  intros ??? oRF.
+  erewrite <-2!wk_fst.
+  unshelve eapply SirrLR, SfstRed, (SwkLR _ _ _ RΣ), Rp.
+  now unshelve eapply RF.
+  all: easy.
 Qed.
-
-(* Lemma fstRed {l Γ} {wfΓ : [|-Γ]} {F F' G G' p p'}
-  (RΣ : [wfΓ ||-<l> tSig F G ≅ tSig F' G'])
-  (RF : [wfΓ ||-<l> F ≅ F'])
-  (Rp : [wfΓ ||-<l> p ≅ p' : _ | RΣ]) :
-  [wfΓ ||-<l> tFst p ≅ tFst p' : _ | RF].
-Proof.
-  eapply (dSplit_bind Rp).
-  intros ??? oRΣ oRp.
-  eapply Wpackrefold.
-  rewrite <- 2!wk_fst.
-  now unshelve eapply SfstRed, Rp.
-Qed. *)
 
 
 Lemma sndRed {l Γ} {wfΓ :[|-Γ]} {F F' G G'} {p p'}
@@ -174,92 +201,45 @@ Proof.
     Unshelve. easy.
 Qed.
 
-(* Lemma fstRed {l Δ} {wfΔ :[|-Δ]} {F F' G G' p p'}
-  (RΣ : [Δ ||-S<l> tSig F G ≅ tSig F' G'])
-  (RF : [wfΔ ||-<l> F ≅ F'])
-  (Rp : [Δ ||-S<l> p ≅ p' : _ | LRSig' (normRedΣ RΣ)]) :
-  [wfΔ ||-<l> tFst p ≅ tFst p' : _ | RF].
-Proof.
-  eapply redSubstTmEq; cycle 1.
-  + eapply redtm_fst, tmr_wf_red; exact (SigRedTmEq.red (SigRedTmEq.redL Rp)).
-  + eapply redtm_fst, tmr_wf_red.
-    eapply redtmwf_conv.
-    1:exact (SigRedTmEq.red (SigRedTmEq.redR Rp)).
-    now escape.
-  + eapply Split_return; intros.
-    now unshelve eapply SirrLR, (SigRedTmEq.eqFst Rp).
-Qed.
-
-Lemma sndRed {l Δ} {wfΔ :[|-Δ]} {F F' G G'} {p p'}
-  (RΣ : [Δ ||-S<l> tSig F G ≅ tSig F' G'])
-  (RΣn := LRSig' (normRedΣ RΣ))
-  (Rp : [Δ ||-S<l> p ≅ p' : _ | RΣn])
-  (RGfstp : [wfΔ ||-<l> G[(tFst p)..] ≅ G'[(tFst p')..]]) :
-  [wfΔ ||-<l> tSnd p ≅ tSnd p' : _ | RGfstp].
-Proof.
-  eapply redSubstTmEq; cycle 1.
-  + eapply redtm_snd, tmr_wf_red; exact (SigRedTmEq.red (SigRedTmEq.redL Rp)).
-  + eapply redtm_snd, tmr_wf_red, redtmwf_conv.
-    1: exact (SigRedTmEq.red (SigRedTmEq.redR Rp)).
-    now escape.
-  + erewrite <-wk_id_ren_on, <-(wk_id_ren_on _ (tSnd (nf (redL _)))).
-    eapply irrLRConv, (SigRedTmEq.eqSnd Rp wk_id wfΔ).
-    eassert (RF : [wfΔ ||-< l> F ≅ F'])
-      by (eapply Split_return; intros;
-      now eapply (normRedΣ RΣ).(PolyRed.shpRed)).
-    erewrite wk_fst, <- eq_subst_scons.
-    epose proof (redTmFwd' Rp) as [Rp' _ _ _ _].
-    epose proof (fstRed := fstRed RΣ RF Rp').
-    symmetry.
-    eapply (dSplit_bind fstRed).
-    intros Ξ wfΞ ρΞ oRF ofstRed.
-    eapply WAdrefold.
-    rewrite 2!subst_ren_subst_mixed.
-    eapply kripkeLRlrefl.
-    - clear dependent Ξ; intros Ξ a b ρΞ wfΞ RAA'.
-      now eapply (normRedΣ RΣ).(PolyRed.posRed).
-    - now unshelve eapply SirrLR, fstRed.
-    Unshelve. easy.
-Qed. *)
 
 Lemma pairFstRed {Γ} {wfΓ :[|-Γ]} {A} {wfA : [Γ |- A]} {A' B B' a a' b b' l}
-  (RA : [wfΓ ||-<l> A ≅ A'])
+  (RA : [Γ ||-S<l> A ≅ A'])
   (RB : [wfc_cons wfΓ wfA ||-<l> B ≅ B'])
   (WtB' : [Γ ,, A' |- B'])
   (RBa : [wfΓ ||-<l> B[a..] ≅ B'[a'..] ])
-  (Ra : [wfΓ ||-<l> a ≅ a' : A | RA])
+  (Ra : [Γ ||-S<l> a ≅ a' : A | RA])
   (Rb : [wfΓ ||-<l> b ≅ b' : _ | RBa ]) :
-  [wfΓ ||-<l> tFst (tPair A B a b) ≅ tFst (tPair A' B' a' b') : _ | RA].
+  [Γ ||-S<l> tFst (tPair A B a b) ≅ tFst (tPair A' B' a' b') : _ | RA].
 Proof.
   escape.
-  eapply redSubstTmEq; tea.
+  eapply SredSubstTmEq; tea.
   1,2: eapply redtm_fst_beta; tea; now eapply ty_conv.
 Qed.
 
 Lemma pairFstRed' {Γ} {wfΓ :[|-Γ]} {A} {wfA : [Γ |- A]} {A' B B' a a' b b' l}
-  (RA : [wfΓ ||-<l> A ≅ A'])
+  (RA : [Γ ||-S<l> A ≅ A'])
   (RB : [wfc_cons wfΓ wfA ||-<l> B ≅ B'])
   (WtB' : [Γ ,, A' |- B'])
   (RBa : [wfΓ ||-<l> B[a..] ≅ B'[a'..] ])
-  (Ra : [wfΓ ||-<l> a ≅ a' : A | RA])
+  (Ra : [Γ ||-S<l> a ≅ a' : A | RA])
   (Rb : [wfΓ ||-<l> b ≅ b' : _ | RBa ]) :
-  [wfΓ ||-<l> tFst (tPair A B a b) ≅ tFst (tPair A' B' a' b') : _ | RA]
-  × [wfΓ ||-<l> tFst (tPair A B a b) ≅ a : _ | lrefl RA]
-  × [wfΓ ||-<l> tFst (tPair A' B' a' b') ≅ a' : _ | urefl RA ].
+  [Γ ||-S<l> tFst (tPair A B a b) ≅ tFst (tPair A' B' a' b') : _ | RA]
+  × [Γ ||-S<l> tFst (tPair A B a b) ≅ a : _ | lrefl RA]
+  × [Γ ||-S<l> tFst (tPair A' B' a' b') ≅ a' : _ | urefl RA ].
 Proof.
   escape.
-  eapply redSubstTmEq'; tea.
+  eapply SredSubstTmEq'; tea.
   1,2: eapply redtm_fst_beta; tea; now eapply ty_conv.
 Qed.
 
 Lemma pairSndRed {Γ} {wfΓ :[|-Γ]} {A} {wfA : [Γ |- A]} {A' B B' a a' b b' l}
-  (RA : [wfΓ ||-<l> A ≅ A'])
+  (RA : [Γ ||-S<l> A ≅ A'])
   (RB : [wfc_cons wfΓ wfA ||-<l> B ≅ B'])
   (WtB' : [Γ ,, A' |- B'])
   (RBa : [wfΓ ||-<l> B[a..] ≅ B'[a'..] ])
   (RBfst : [wfΓ ||-<l> B[(tFst (tPair A B a b))..] ≅ B'[(tFst (tPair A' B' a' b'))..]])
   (RBfsta : [wfΓ ||-<l> B[a..] ≅ B[(tFst (tPair A B a b))..]])
-  (Ra : [wfΓ ||-<l> a ≅ a' : A | RA])
+  (Ra : [Γ ||-S<l> a ≅ a' : A | RA])
   (Rb : [wfΓ ||-<l> b ≅ b' : _ | RBa ]) :
   [wfΓ ||-<l> tSnd (tPair A B a b) ≅ tSnd (tPair A' B' a' b') : _ | RBfst ].
 Proof.
@@ -269,167 +249,101 @@ Proof.
   1,2: eapply redtm_snd_beta; tea; now eapply ty_conv.
 Qed.
 
-Lemma canonSig {Γ A A' B B' l p p'}
-  {RΣ : [Γ ||-S< l > tSig A B ≅ tSig A' B']} :
-  [ Γ ||-S< l > p ≅ p' : tSig A B | RΣ] ->
-  [ Γ ||-S< l > p ≅ p' : tSig A B | LRSig' (normRedΣ RΣ)].
-Proof.
-  intro. now eapply SirrLR.
-Qed.
-
-Lemma sigEtaRed' {Γ} {wfΓ : [|-Γ]} {A A' B B' l p p'}
+Lemma sigEtaRed {Γ} {wfΓ : [|-Γ]} {A A' B B' l p p'}
   (RΣ : [Γ ||-S<l> tSig A B ≅ tSig A' B'])
-  (RΣ' : [wfΓ ||-<l> tSig A B ≅ tSig A' B'])
-  (RA : [wfΓ ||-<l> A ≅ A'])
+  (RA : [Γ ||-S<l> A ≅ A'])
   (RBfst : [wfΓ ||-<l> B[(tFst p)..] ≅ B'[(tFst p')..]])
   (Rp : [Γ ||-S<l> p : _ | RΣ])
   (Rp' : [Γ ||-S<l> p' : _ | RΣ])
-  (Rfstpp' : [wfΓ ||-<l> tFst p ≅ tFst p' : _ | RA])
+  (Rfstpp' : [Γ ||-S<l> tFst p ≅ tFst p' : _ | RA])
   (Rsndpp' : [wfΓ ||-<l> tSnd p ≅ tSnd p' : _ | RBfst]) :
-  [wfΓ ||-<l> p ≅ p' : _ | RΣ'].
+  [Γ ||-S<l> p ≅ p' : _ | RΣ].
 Proof.
   eapply canonSig in Rp, Rp'.
-  eapply SigRedTmEq_from in Rp, Rp'.
-  pose proof (redTmFwd' Rp) as [Rpnf _ _ _ _]; pose proof (Rpnf1 := fstRed _ RA Rpnf).
-  pose proof (redTmFwd' Rp) as [Rpnf' _ _ _ _]; pose proof (Rpnf1' := fstRed _ RA Rpnf').
-  unshelve eapply (build_sigRedTmEq' _ Rp.(SigRedTmEq'.redL _  _ _) Rp'.(redL)).
-  
-
-Lemma sigEtaRed {Γ} {wfΓ : [|-Γ]} {A A' B B' l p p'}
-  (RΣ : [wfΓ ||-<l> tSig A B ≅ tSig A' B'])
-  (RA : [wfΓ ||-<l> A ≅ A'])
-  (RBfst : [wfΓ ||-<l> B[(tFst p)..] ≅ B'[(tFst p')..]])
-  (Rp : [wfΓ ||-<l> p : _ | RΣ])
-  (Rp' : [wfΓ ||-<l> p' : _ | RΣ])
-  (Rfstpp' : [wfΓ ||-<l> tFst p ≅ tFst p' : _ | RA])
-  (Rsndpp' : [wfΓ ||-<l> tSnd p ≅ tSnd p' : _ | RBfst]) :
-  [wfΓ ||-<l> p ≅ p' : _ | RΣ].
-Proof.
-  eapply (dSplit_bind Rp).
-  intros ??? _ oRp.
-  eapply Wpackrefold.
-  eapply (dSplit_wk_bind Rp' ρ).
-  intros ?? ρΞ oRΣ oRp'.
-  eapply Wpackrefold.
-  pose proof (Rp0 := cover Rp Ξ wfΞ (ρΞ∘w ρ) (overtree_PSh Rp oRp) oRΣ); cbn in Rp0.
-  pose proof (Rp'0 := cover Rp' Ξ wfΞ (ρΞ∘w ρ) oRp' oRΣ); cbn in Rp'0.
-  set (RΣ0 := cover RΣ Ξ wfΞ (ρΞ ∘w ρ) oRΣ) in *; clearbody RΣ0. cbn in RΣ0.
-  pose proof (RA' := WwkRed (wkLR _ _ _ _ RA) (ρΞ∘w ρ) wfΞ).
-  pose proof (redTmFwd' (canonSig Rp0)) as [Rpnf _ _ _ _]; pose proof (Rpnf1 := fstRed _ RA' Rpnf).
-  pose proof (redTmFwd' (canonSig Rp'0)) as [Rpnf' _ _ _ _]; pose proof (Rpnf1' := fstRed _ RA' Rpnf').
-  eapply (irrLREq (A:= tSig A⟨ρΞ∘w ρ⟩ B ⟨wk_up A (ρΞ∘w ρ)⟩)).
-  1: symmetry; eapply wk_comp_ren_on.
-  rewrite 2!wk_comp_ren_on.
-  eapply Wpack_return.
-  unshelve eapply (build_sigRedTmEq' _ (canonSig Rp0).(redL) (canonSig Rp'0).(redL)).
-  easy.
-  + 
-
-Lemma sigEtaRed {Γ} {wfΓ :[|-Γ]} {A A' B B' l p p'}
-  (RΣ0 : [Γ ||-S<l> tSig A B ≅ tSig A' B'])
-  (RΣn := normRedΣ RΣ0)
-  (RΣ := (LRSig' RΣn))
-  (RA : [wfΓ ||-<l> A ≅ A'])
-  (RBfst : [wfΓ ||-<l> B[(tFst p)..] ≅ B'[(tFst p')..]])
-  (Rp : [Γ ||-<l> p : _ | RΣ])
-  (Rp' : [Γ ||-<l> p' : _ | RΣ])
-  (Rfstpp' : [wfΓ ||-<l> tFst p ≅ tFst p' : _ | RA])
-  (Rsndpp' : [wfΓ ||-<l> tSnd p ≅ tSnd p' : _ | RBfst]) :
-  [wfΓ ||-<l> p ≅ p' : _ | WAd_return (wfΓ := wfΓ) RΣ].
-Proof.
-  pose proof (redTmFwd' Rp) as [Rpnf _ _ _ _]; pose proof (Rpnf1 := fstRed _ RA Rpnf).
-  pose proof (redTmFwd' Rp') as [Rpnf' _ _ _ _]; pose proof (Rpnf1' := fstRed _ RA Rpnf').
-  eapply (dSplit_bind Rpnf1).
-  intros ??? oRA oRpnf1.
-  unshelve eapply Wpackrefold.
-  1: now eapply WAd_return, SwkLR.
-  eapply (dSplit_wk_bind_return Rpnf1' ρ).
-  intros ?? ρΞ oRA' oRpnf1' oirr.
-  unshelve eapply SirrLREq; clear oirr.
-  4: symmetry; eapply wk_comp_ren_on.
-  2: now eapply SwkLR.
   eapply SirrLR.
-  eapply (build_sigRedTmEq'); fold ren_term.
-  change (tSig A B)⟨ρ' ∘w ρ⟩ with (tSig A⟨ρ' ∘w ρ⟩ B⟨ρ' ∘w ρ⟩)
-  rewrite 
-  unshelve eapply Wpack_return, SwkLR, (build_sigRedTmEq' _ Rp.(redL) Rp'.(redL)); tea.
-  - transitivity (tFst p); [symmetry|transitivity (tFst p')]; eapply SirrLR.
-    eapply Rpnf1.
-  - pose proof (RBB' := instKripkeSubst RΣn.(PolyRed.posRed)).
-    pose proof (RB := instKripkeSubst (kripkeLRlrefl RΣn.(PolyRed.posRed))).
-    pose proof (RB' := instKripkeSubst (kripkeLRurefl RΣn.(PolyRed.posRed))).
+  pose proof (redTmFwd' Rp) as [Rpnf _ _ _ _]; pose proof (Rpnf1 := SfstRed _ RA Rpnf).
+  pose proof (redTmFwd' Rp') as [Rpnf' _ _ _ _]; pose proof (Rpnf1' := SfstRed _ RA Rpnf').
+  unshelve eapply (build_sigRedTmEq' _ Rp.(redL) Rp'.(redL)); tea.
+  - transitivity (tFst p); [symmetry|transitivity (tFst p')]; now eapply SirrLR.
+  - set (RΣn := normRedΣ RΣ).
+    pose proof (RBB' := instKripkeSubst wfΓ RΣn.(PolyRed.posRed)).
+    pose proof (RB := instKripkeSubst wfΓ (kripkeLRlrefl (wfΓ :=wfΓ) RΣn.(PolyRed.posRed))).
     pose proof (RBpnf1 := RBB' _ _ _ Rpnf1); pose proof (sndRed _ Rpnf RBpnf1).
     pose proof (RBpnf1' := RBB' _ _ _ Rpnf1'); pose proof (sndRed _ Rpnf' RBpnf1').
-    cbn in *; eapply irrLR.
-    eapply ((transLR _ _).(transRedTm) _ (tSnd p)).
+    cbn -[Wpack] in *; eapply irrLR.
+    transitivity (tSnd p).
     1: symmetry; eapply irrLRConv; tea; exact (RB _ _ _ Rpnf1).
-    eapply ((transLR _ _).(transRedTm) _ (tSnd p')); tea.
+    transitivity (tSnd p').
+    1: eapply irrLRConv; tea; exact (RB _ _ _ Rpnf1).
     eapply irrLRConv; [|tea].
-    eapply RBB', urefl; tea.
+    eapply RB.
+    transitivity (tFst p); tea.
+    1:symmetry; tea.
     Unshelve.
-    3: eapply RB', urefl; tea.
-    eapply RB; now symmetry.
+    2: eapply RB; symmetry; tea.
 Qed.
 
 
-Lemma mkPair_isLRPair {Γ A A' A1 B B' B1 a1 b1 l}
-  (RΣ0 : [Γ ||-<l> tSig A B ≅ tSig A' B'])
+Lemma mkPair_isLRPair {Γ} {wfΓ : [|-Γ]} {A A' A1 B B' B1 a1 b1 l}
+  (RΣ0 : [Γ ||-S<l> tSig A B ≅ tSig A' B'])
   (RΣ := normRedΣ RΣ0)
-  (RA1 : [Γ ||-<l> A ≅ A1])
-  (RB1 : [Γ ||-<l> B[a1..] ≅ B1[a1..]])
-  (Ra1 : [Γ ||-<l> a1 : _ | RA1])
-  (Rb1 : [Γ ||-<l> b1 : _ | RB1])
+  (RA1 : [Γ ||-S<l> A ≅ A1])
+  (RB1 : [wfΓ ||-<l> B[a1..] ≅ B1[a1..]])
+  (Ra1 : [Γ ||-S<l> a1 : _ | RA1])
+  (Rb1 : [wfΓ ||-<l> b1 : _ | RB1])
 : isLRPair RΣ (tPair A1 B1 a1 b1).
 Proof.
   escape.
   unshelve eapply PairLRPair; tea; intros.
-  - now unshelve now eapply irrLR, wkLR.
+  - now unshelve now eapply SirrLR, SwkLR.
   - now unshelve now eapply irrLREq, wkLR; tea; rewrite subst_ren_subst_mixed.
 Qed.
 
-Definition pairSigRedTm {Γ A A' A1 B B' B1 a1 b1 l}
-  (RΣ0 : [Γ ||-<l> tSig A B ≅ tSig A' B'])
-  (RΣ1 : [Γ ||-<l> tSig A B ≅ tSig A1 B1])
+Definition pairSigRedTm {Γ} {wfΓ : [|-Γ]} {A A' A1 B B' B1 a1 b1 l}
+  (RΣ0 : [Γ ||-S<l> tSig A B ≅ tSig A' B'])
+  (RΣ1 : [Γ ||-S<l> tSig A B ≅ tSig A1 B1])
   (RΣ := normRedΣ RΣ0)
-  (Ra1 : [Γ ||-<l> a1 : _ | redΣdom RΣ0])
-  (Rb1 : [Γ ||-<l> b1 : _ | redΣcodfst RΣ0 Ra1])
+  (Ra1 : [Γ ||-S<l> a1 : _ | SredΣdom RΣ0])
+  (Rb1 : [wfΓ ||-<l> b1 : _ | redΣcodfst (wfΓ:=wfΓ) RΣ0 Ra1])
 : SigRedTm RΣ (tPair A1 B1 a1 b1).
 Proof.
-  exists (tPair A1 B1 a1 b1); pose proof (RA := redΣdom RΣ1);
-    pose proof (RB := redΣcodfst RΣ1 (fst (irrLR _ RA _ _) Ra1)).
+  exists (tPair A1 B1 a1 b1); pose proof (RA := SredΣdom RΣ1);
+    pose proof (RB := redΣcodfst (wfΓ:=wfΓ) RΣ1 (fst (SirrLR _ RA _ _) Ra1)).
   + eapply redtmwf_refl; cbn.
-    assert (wfΓ : [|- Γ]) by (escape ; gtyping).
-    assert [_ ||-<l> a1 : _ | urefl RA ] by now eapply irrLRConv.
-    pose proof (instKripkeFamConv wfΓ (normRedΣ RΣ1).(PolyRed.posRed)).
+    eassert (wfA1 : [Γ|-A1]) by (escape; gtyping).
+    assert [_ ||-S<l> a1 : _ | urefl RA ] by now eapply SirrLRConv.
+    pose proof (instKripkeFamConv wfΓ wfA1 (normRedΣ RΣ1).(PolyRed.posRed)).
     assert [_ ||-<l> b1 : _ | urefl RB ] by now eapply irrLRConv.
     escape.
     eapply ty_conv; [ eapply ty_pair; tea| now symmetry].
-  + now unshelve now eapply mkPair_isLRPair; eapply irrLR.
+  + now unshelve now eapply mkPair_isLRPair; [eapply SirrLR | eapply irrLR].
 Defined.
 
-Lemma pairCongRed {Γ A A' B B' a a' b b' l}
-  (RΣ0 : [Γ ||-<l> tSig A B ≅ tSig A' B'])
-  (RΣ := normRedΣ RΣ0)
-  (RΣ' := LRSig' RΣ)
-  (RA : [Γ ||-<l> A ≅ A'])
-  (RBa : [Γ ||-<l> B[a..] ≅ B'[a'..] ])
-  (Ra : [Γ ||-<l> a ≅ a' : A | RA])
-  (Rb : [Γ ||-<l> b ≅ b' : _ | RBa ]) :
-  [Γ ||-<l> tPair A B a b ≅ tPair A' B' a' b' : _ | RΣ'].
+Lemma pairCongRed {Γ} {wfΓ : [|-Γ]} {A A' B B' a a' b b' l}
+  (RΣ : [Γ ||-S<l> tSig A B ≅ tSig A' B'])
+(*   (RΣ := normRedΣ RΣ0)
+  (RΣ' := LRSig' RΣ) *)
+  (RA : [Γ ||-S<l> A ≅ A'])
+  (RBa : [wfΓ ||-<l> B[a..] ≅ B'[a'..] ])
+  (Ra : [Γ ||-S<l> a ≅ a' : A | RA])
+  (Rb : [wfΓ ||-<l> b ≅ b' : _ | RBa ]) :
+  [Γ ||-S<l> tPair A B a b ≅ tPair A' B' a' b' : _ | RΣ].
 Proof.
-  assert (wfΓ : [|-Γ]) by (escape; gtyping).
-  pose proof (convtyB := redΣcod RΣ').
-  pose proof (wtB' := escape (symmetry (instKripkeFamConv wfΓ RΣ.(PolyRed.posRed)))).
+  assert (wfA : [Γ|-A]) by (escape; gtyping).
+  assert (wfA' : [Γ|-A']) by (escape; gtyping).
+(*   eapply canonSig. *)
+  pose proof (convtyB := redΣcod (wfΓ:=wfΓ) (wfF:=wfA) RΣ).
+  pose proof (wtB' := fst (escapeSplitTy (symmetry (instKripkeFamConv wfΓ wfA' (normRedΣ RΣ).(PolyRed.posRed))))).
   unshelve epose proof (pairFstRed' RA convtyB wtB' RBa Ra Rb) as (ff'&fa&fa').
-  pose proof (RBconv := instKripkeSubst (kripkeLRlrefl RΣ.(PolyRed.posRed)) RA (fst (irrLR _ _ _ _) fa)).
-
-  unshelve eapply build_sigRedTmEq'.
-  + unshelve eapply pairSigRedTm; eapply lrefl; tea; now eapply irrLR.
-  + unshelve eapply pairSigRedTm; tea; eapply urefl. now eapply irrLR.
-    eapply irrLRConv; tea; eapply (instKripkeSubst (kripkeLRlrefl RΣ.(PolyRed.posRed)) RA Ra).
-  + cbn; eapply irrLR, pairFstRed; tea.
-  + unshelve now cbn; eapply irrLR; eapply pairSndRed; tea; symmetry.
-    now eapply (instKripkeSubst RΣ.(PolyRed.posRed)).
+  pose proof (RBconv := instKripkeSubst wfΓ (kripkeLRlrefl (wfΓ:=wfΓ) (normRedΣ RΣ).(PolyRed.posRed)) RA (fst (SirrLR _ _ _ _) fa)).
+  eapply canonSig_inv.
+  unshelve eapply build_sigRedTmEq'; tea.
+  + unshelve eapply pairSigRedTm; tea; eapply lrefl; tea; [eapply SirrLR|eapply irrLR]; tea.
+  + unshelve eapply pairSigRedTm; tea; eapply urefl. now eapply SirrLR.
+    eapply irrLRConv; tea; eapply (instKripkeSubst wfΓ (kripkeLRlrefl (wfΓ:=wfΓ) (normRedΣ RΣ).(PolyRed.posRed)) RA Ra).
+  + cbn; eapply SirrLR, pairFstRed; tea.
+  + unshelve now cbn -[Wpack]; eapply irrLR, pairSndRed; tea; symmetry.
+    now eapply (instKripkeSubst wfΓ (normRedΣ RΣ).(PolyRed.posRed)).
 Qed.
 
 End SigmaRed.
